implement hashing

Luatable/Basic.lean
@@ -1,1 +1,104 @@
-def hello := "world"
+import Mathlib.Data.Vector.Basic
+
+abbrev TBoolean := Bool
+abbrev TNumber := UInt64 -- Using this for now becuse Float is very cumbersome to use
+
+structure TString where
+  hash : Nat
+  size : Nat
+
+inductive TObject where
+  | string (str: TString)
+  | number (n: TNumber) -- Up to Lua 5.2, Lua exclusively used doubles for numbers
+  | nil
+  | bool (b: TBoolean)
+  | light_user_value (pointer: USize)
+
+structure Node where
+  key: TObject
+  val: TObject
+
+structure Table where
+  limit : Nat
+  array : List TValue
+  node : List Node
+  metatable: Table
+
+def maxBits := 24
+def tooBig (x : UInt32) : Bool := (x - 1) >>> maxBits.toUInt32 ≠ 0
+
+def TNumber.nthByte (x i : TNumber) : TNumber :=
+  x <<< i &&& 0xff
+
+def TNumber.memcpy (x: TNumber) : List UInt8 :=
+  List.range' 0 8 8 |>.map Nat.toUInt64 |>.map x.nthByte |>.map UInt64.toUInt8
+
+def lmod (s size : Nat) := s &&& (size - 1)
+
+lemma Nat.or_one (x : Nat) : x ||| 1 ≤ x + 1 := by sorry
+lemma Nat.or_one_pos (x : Nat) : x ||| 1 > 0 := by sorry
+
+namespace Table
+
+def lsizenode (t : Table) : Nat := t.node.length.log2
+def sizenode (t : Table) : Nat := 2 ^ t.lsizenode
+
+
+def hashpow2 (t: Table) (n: Nat) (node_exists : t.node.length > 0) : Node :=
+  t.node[lmod n t.sizenode]'
+  (by
+    rw[lmod, sizenode, lsizenode]
+    simp
+    calc
+      n % 2 ^ t.node.length.log2 < 2 ^ t.node.length.log2 := by
+        apply Nat.mod_lt
+        exact Nat.two_pow_pos t.node.length.log2
+      _ ≤ t.node.length := by
+        apply Nat.log2_self_le
+        exact Nat.not_eq_zero_of_lt node_exists)
+
+def hashmod (t: Table) (n: Nat) (node_exists : t.node.length > 0): Node :=
+  t.node[n % ((t.sizenode - 1) ||| 1)]'
+  (by
+    have h : t.sizenode - 1 ||| 1 < t.node.length := by
+      sorry
+    calc
+      n % (t.sizenode - 1 ||| 1) < t.sizenode - 1 ||| 1 := by
+        apply n.mod_lt
+        exact Nat.or_one_pos (t.sizenode - 1)
+      _ < t.node.length := h)
+
+class Hashable (α : Type) where
+  hashnode (val : α) (t : Table) (node_exists : t.node.length > 0) : Node
+
+instance : Hashable TString where
+  hashnode := λ str t ex ↦ t.hashpow2 str.hash ex
+
+instance : Hashable TNumber where
+  hashnode := λ n t ex ↦  t.hashmod (n + 1).memcpy.sum.toNat ex
+
+instance : Hashable TBoolean where
+  hashnode := λ b t ex ↦ t.hashpow2 b.toNat ex
+
+instance : Hashable USize where
+  hashnode := λ p t ex ↦ t.hashmod p.toUInt32.toNat ex
+
+def mainPosition (t : Table) (key : TObject) : Node :=
+  match key with
+  | TObject.string str => Hashable.hashnode str t sorry
+  | TObject.number n => Hashable.hashnode n t sorry
+  | TObject.bool b => Hashable.hashnode b t sorry
+  | TObject.light_user_value p => Hashable.hashnode p t sorry
+  | _ => sorry
+
+def arrayIndex (key: TObject) : Option UInt32 :=
+  match key with
+  | TObject.number n =>
+    let rounded := n.toUInt32
+    if rounded >= 1 ∧ ¬tooBig rounded then
+      some rounded
+    else
+      none
+  | _ => none
+
+end Table
